src/PlutusIR/Transform/Unwrap.v
@@ -1,6 +1,6 @@
 From PlutusCert Require Import
   PlutusIR
-  Transform.Congruence
+  Transform.Compat
 .
 
 Import NamedTerm.
@@ -13,8 +13,8 @@ Inductive unwrap_cancel : Term -> Term -> Prop :=
       t ▷-unwrap t' ->
       Unwrap (IWrap ty1 ty2 t) ▷-unwrap t'
 
-  | uc_cong : forall t t',
-      Cong unwrap_cancel t t' ->
+  | uc_compat : forall t t',
+      Compat unwrap_cancel t t' ->
       t ▷-unwrap t'
 
   where "t1 ▷-unwrap t2" := (unwrap_cancel t1 t2)
